Start proof

r1cs.v
@@ -1,25 +1,33 @@
 Require Import
         String
-        Nat
+        Coq.ZArith.ZArith
+        Coq.ZArith.BinIntDef
         Coq.Init.Datatypes
         Coq.FSets.FMapList
         Coq.Structures.OrderedTypeEx.
 
-Module Import M := FMapList.Make(String_as_OT).
-Open Scope string_scope.
+Print Z.
+Locate of_nat.
+Open Scope Z_scope.
 
-Definition Env := M.t nat.
-Definition Clean := empty nat.
+Module L := Coq.Lists.List.
+Module M := FMapList.Make(String_as_OT).
+
+Open Scope string_scope.
+Set Implicit Arguments.
+
+Definition Env := M.t Z.
+Definition Clean := M.empty Z.
 
 Section R1C.
   (** Finite field modulo prime P *)
-  Parameter P: nat.
-  Parameter (H: forall n: nat, Nat.modulo P n = 0).
+  Parameter P: Z.
+  Parameter (H: forall n: Z, Z.modulo P n = 0).
 
   (** ADT for R1Constraint *)
   Inductive R1C :=
-  | Const (n: nat)
-  | Mult (n: nat) (v: string)
+  | Const (n: Z)
+  | Mult (n: Z) (v: string)
   | Neg (inner: R1C)
   | Plus (left: R1C) (right: R1C).
 
@@ -29,7 +37,7 @@ Section R1C.
   Declare Scope r1c_scope.
   Bind Scope r1c_scope with R1C.
   Open Scope r1c_scope.
-  Coercion Const : nat >-> R1C.      
+  Coercion Const : Z >-> R1C.      
   Definition string_to_r1c(s: string) := Mult 1 s.
   Coercion string_to_r1c: string >-> R1C.
 
@@ -39,11 +47,25 @@ Section R1C.
   Notation "e1 == e2" := (Plus e1 (Neg e2)) (at level 55, left associativity): r1c_scope.
 
   (** Let's try it out *)
-  Compute "r0"  == 0 + 1.
+  Definition ex1_equation := "r0"  == 0 + 1.
+
+  Fixpoint substitute(env: Env)(constr: R1C) : option Z :=
+    match constr with
+    | Mult n v => match M.find v env with
+                 | None => None
+                 | Some v' => Some (Z.mul n v')
+                 end
+    | Plus l r => match substitute env l, substitute env r with
+                 | Some a, Some b => Some (Z.add a b)
+                 | _, _ => None
+                 end
+    | Neg i => option_map Z.opp (substitute env i)
+    | Const n => Some n
+    end.
 
   (** Check a valuation satisfies an R1CS *)
-  Definition check(env: Env)(C: R1CS): Prop.
-    Admitted.
+  Definition check(env: Env)(C: R1CS): Prop := L.Forall (fun r1c => substitute env r1c = Some 0) C.
+  
 End R1C.
 
 Section Expr.
@@ -55,43 +77,60 @@ Section Expr.
   | AAdd (dst: string) (src: string)
   | ASub (dst: string) (src: string)
   | AMult (dst: string) (src: string)
-  | AMov (dst: string) (const: nat)
+  | AMov (dst: string) (const: Z)
   | ASeq (head: AsmExpr) (tail: AsmExpr).
 
-  Infix "|" := ASeq (at level 55): asm_scope.
+  Infix ";;" := ASeq (at level 55): asm_scope.
   Bind Scope asm_scope with AsmExpr.
   
   (** Program: r0 <- 0 + 1 *)
-  Compute AMov "%r0" 0
-          | AMov "%r1" 1
-          | AAdd "%r0" "%r1".
-    
-  Definition eval(env: Env)(p: AsmExpr): Env :=
+  Definition ex1_prog :=
+    AMov "%r0" 0 ;;
+    AMov "%r1" 1 ;;
+    AAdd "%r0" "%r1".
+
+  Fixpoint eval(env: Env)(p: AsmExpr): Env :=
     match p with
-    | AAdd l r => match (find l env, find r env) with
-                 | (Some lv, Some rv) => add l (lv + rv) env
-                 | (None, Some rv) => add l rv env
-                 | _ => None
+    | AAdd l r => match M.find l env, M.find r env with
+                 | Some lv, Some rv => M.add l (lv + rv) env
+                 | None, Some rv => M.add l rv env
+                 | _, _ => env
                  end
-    | ASub l r => match (find l env, find r env) with
-                 | (Some lv, Some rv) => add l (lv - rv) env
-                 | _ => None
+    | ASub l r => match M.find l env, M.find r env with
+                 | Some lv, Some rv => M.add l (lv - rv) env
+                 | _, _ => env
                  end
-    | AMult r v => match (find l env, find r env) with
-                 | (Some lv, Some rv) => add l (lv * rv) env
-                 | _ => None
+    | AMult l r => match M.find l env, M.find r env with
+                  | Some lv, Some rv => M.add l (lv * rv) env
+                  | _, _ => env
                   end
-    | AMov reg v => add reg v env
+    | AMov reg v => M.add reg v env
     | ASeq a b => eval (eval env a) b
     end.
   
 End Expr.
 
-Set Implicit Arguments.
+Require Import Coq.FSets.FMapFacts.
+
+Module P := WProperties_fun String_as_OT M.
+Module F := P.F.
 
 Section AbstrInterp.
 
-  Definition simulation(P: AsmExpr)(C: R1CS) := forall (env: map string nat),
-      env = nil -> let endState := eval env P in check endState C.
-           
+  Definition simulation_correct(P: AsmExpr)(C: R1CS) := forall (env: Env),
+    let endState := eval env P in check endState C.
+
+  Theorem some_example_correct:
+    simulation_correct ex1_prog (L.cons ex1_equation L.nil).
+  Proof.
+    unfold simulation_correct.
+    intros.
+    simpl.
+    replace (
+    rewrite F.add_eq_o.
+  Admitted.
   
+    
+    rewrite F.add_eq_o.
+    F.map_iff
+End AbstrInterp.
